Add transparency opt for forward/destruct builders

Aesop/Builder/Forward.lean
@@ -14,6 +14,11 @@ namespace Aesop
 structure ForwardBuilderOptions extends RegularBuilderOptions where
   immediateHyps : Option (Array Name)
   clear : Bool
+  /-- The transparency used by the rule tactic. -/
+  transparency : TransparencyMode
+  /-- The transparency used to index the rule. The rule is not indexed unless
+  this is `.reducible`. -/
+  indexTransparency : TransparencyMode
   deriving Inhabited
 
 protected def ForwardBuilderOptions.default (clear : Bool) :
@@ -21,20 +26,22 @@ protected def ForwardBuilderOptions.default (clear : Bool) :
   toRegularBuilderOptions := .default
   immediateHyps := none
   clear := clear
+  transparency := .default
+  indexTransparency := .reducible
 
 namespace RuleBuilder
 
-def getImmediatePremises (name : Name) (type : Expr) : Option (Array Name) →
-    MetaM (UnorderedArraySet Nat)
-  | none => do
+def getImmediatePremises (name : Name) (type : Expr) (md : TransparencyMode) :
+    Option (Array Name) → MetaM (UnorderedArraySet Nat)
+  | none =>
     -- If no immediate names are given, every argument becomes immediate,
     -- except instance args and dependent args.
-    forallTelescopeReducing type λ args _ => do
+    withTransparency md $ forallTelescopeReducing type λ args _ => do
       if args.isEmpty then
         throwError "aesop: while registering '{name}' as a forward rule: not a function"
       let mut result := #[]
       for h : i in [:args.size] do
-        have h : i < args.size := by simp_all [Membership.mem]
+        have h : i < args.size := h.2
         let fvarId := args[i].fvarId!
         let ldecl ← fvarId.getDecl
         let isNondep : MetaM Bool :=
@@ -43,10 +50,10 @@ def getImmediatePremises (name : Name) (type : Expr) : Option (Array Name) →
         if ← pure ! ldecl.binderInfo.isInstImplicit <&&> isNondep then
           result := result.push i
       return UnorderedArraySet.ofDeduplicatedArray result
-  | some immediate => do
+  | some immediate =>
     -- If immediate names are given, we check that corresponding arguments
     -- exists and record these arguments' positions.
-    forallTelescopeReducing type λ args _ => do
+    withTransparency md $ forallTelescopeReducing type λ args _ => do
       let mut unseen := immediate.sortAndDeduplicate (ord := ⟨Name.quickCmp⟩)
       let mut result := #[]
       for h : i in [:args.size] do
@@ -59,42 +66,51 @@ def getImmediatePremises (name : Name) (type : Expr) : Option (Array Name) →
         "aesop: while registering '{name}' as a forward rule: function does not have arguments with these names: '{unseen}'"
       return UnorderedArraySet.ofDeduplicatedArray result
 
-private def getIndexingMode (type : Expr) (immediate : UnorderedArraySet Nat) :
-    MetaM IndexingMode := do
+private def getIndexingMode (type : Expr) (immediate : UnorderedArraySet Nat)
+    (md : TransparencyMode) : MetaM IndexingMode := do
   let immediate := immediate.toArray
   match immediate.max? with
   | some i =>
     withoutModifyingState do
-      let (args, _, _) ← forallMetaTelescopeReducing type
+      let (args, _, _) ← withTransparency md $ forallMetaTelescopeReducing type
       match args.get? i with
       | some arg =>
-        let argT ← inferType arg
+        let argT := (← arg.mvarId!.getDecl).type
         let keys ← DiscrTree.mkPath argT
         return .hyps keys
       | none => throwError
         "aesop: internal error: immediate arg for forward rule is out of range"
   | none => return .unindexed
 
-def forward (opts : ForwardBuilderOptions) : RuleBuilder := λ input =>
+def forward (opts : ForwardBuilderOptions) : RuleBuilder := λ input => do
+  if let .all := opts.transparency then
+    throwError "aesop: forward builder currently does not support transparency 'all'"
   match input.kind with
   | .global decl => do
     let type := (← getConstInfo decl).type
-    let immediate ← getImmediatePremises decl type opts.immediateHyps
-    let tac := .forwardConst decl immediate opts.clear
+    let immediate ←
+      getImmediatePremises decl type opts.transparency opts.immediateHyps
+    let tac := .forwardConst decl immediate opts.clear opts.transparency
     .global <$> mkResult tac type immediate
   | .«local» fvarUserName goal => do
     goal.withContext do
       let type ← instantiateMVars (← getLocalDeclFromUserName fvarUserName).type
-      let immediate ← getImmediatePremises fvarUserName type opts.immediateHyps
-      let tac := .forwardFVar fvarUserName immediate opts.clear
+      let immediate ←
+        getImmediatePremises fvarUserName type opts.transparency
+          opts.immediateHyps
+      let tac := .forwardFVar fvarUserName immediate opts.clear opts.transparency
       .«local» goal <$> mkResult tac type immediate
   where
     mkResult (tac : RuleTacDescr) (type : Expr)
-        (immediate : UnorderedArraySet Nat) : MetaM RuleBuilderResult :=
+        (immediate : UnorderedArraySet Nat) : MetaM RuleBuilderResult := do
+      let indexingMode ← opts.getIndexingModeM do
+        if opts.indexTransparency != .reducible then
+          return .unindexed
+        else
+          getIndexingMode type immediate opts.transparency
       return .regular {
         builder := .forward
-        indexingMode := ← opts.getIndexingModeM $ getIndexingMode type immediate
-        tac
+        tac, indexingMode
       }
 
 end Aesop.RuleBuilder
