Aesop/Util/Basic.lean
@@ -191,16 +191,33 @@ def isAppOfUpToDefeq (f : Expr) (e : Expr) : MetaM Bool :=
 
 section TransparencySyntax
 
-def withTransparencySyntax [Monad m] [MonadQuotation m] (md : TransparencyMode)
-    (k : TSyntax `tactic) : m (TSyntax `tactic) :=
+variable [Monad m] [MonadQuotation m]
+
+open Parser.Tactic
+
+def withTransparencySeqSyntax (md : TransparencyMode)
+    (k : TSyntax ``tacticSeq) : m (TSyntax ``tacticSeq) :=
+  match md with
+  | .default => return k
+  | .all => `(tacticSeq| with_unfolding_all $k)
+  | .reducible => `(tacticSeq| with_reducible $k)
+  | .instances => `(tacticSeq| with_reducible_and_instances $k)
+
+def withAllTransparencySeqSyntax (md : TransparencyMode)
+    (k : TSyntax ``tacticSeq) : m (TSyntax ``tacticSeq) :=
+  match md with
+  | .all => `(tacticSeq| with_unfolding_all $k)
+  | _ => return k
+
+def withTransparencySyntax (md : TransparencyMode) (k : TSyntax `tactic) :
+    m (TSyntax `tactic) :=
   match md with
   | .default   => return k
   | .all       => `(tactic| with_unfolding_all $k:tactic)
   | .reducible => `(tactic| with_reducible $k:tactic)
   | .instances => `(tactic| with_reducible_and_instances $k:tactic)
 
-def withAllTransparencySyntax [Monad m] [MonadQuotation m]
-    (md : TransparencyMode) (k : TSyntax `tactic) :
+def withAllTransparencySyntax (md : TransparencyMode) (k : TSyntax `tactic) :
     m (TSyntax `tactic) :=
   match md with
   | .all  => `(tactic| with_unfolding_all $k:tactic)
