AesopTest/ForwardTransparency.lean
@@ -1,0 +1,32 @@
+/-
+Copyright (c) 2023 Jannis Limperg. All rights reserved.
+Released under Apache 2.0 license as described in the file LICENSE.
+Authors: Jannis Limperg
+-/
+
+import Aesop
+
+set_option aesop.check.all true
+
+def T := Unit → Empty
+
+example (h : T) (u : Unit) : α := by
+  fail_if_success aesop (options := { terminal := true })
+  fail_if_success aesop (add (forward (transparency := reducible)) safe h)
+    (options := { terminal := true })
+  aesop (add forward safe h)
+
+def U := Unit
+
+example (h : T) (u : U) : α := by
+  fail_if_success aesop (options := { terminal := true })
+  fail_if_success aesop (add (forward (transparency := reducible)) safe h)
+    (options := { terminal := true })
+  fail_if_success aesop (add forward safe h) (options := { terminal := true })
+  aesop (add (forward (transparency! := default)) safe h)
+
+abbrev V := Unit
+
+example (h : Unit → Empty) (u : V) : α := by
+  fail_if_success aesop (options := { terminal := true })
+  aesop (add (forward (transparency := reducible)) safe h)
